test/stdlib/test_mem.c
@@ -1,0 +1,160 @@
+#include <assert.h>
+#include <inttypes.h>
+#include <stdbool.h>
+#include <stddef.h>
+#include <stdio.h>
+#include <stdlib.h>
+#include <string.h>
+
+#include "macros.h"
+#include "params.h"
+#include "print.h"
+#include "randombytes.h"
+#include "utils.h"
+
+#ifndef TESTS
+#define TESTS 1000
+#endif
+
+#ifndef IMPL
+#error IMPL not defined
+#endif
+
+#ifndef MAX_BUFSIZE
+#define MAX_BUFSIZE 1024
+#endif
+
+extern void memset_zero_u8_jazz(uint8_t *);
+extern void memset_u8_ptr_jazz(uint8_t *, size_t, uint8_t);
+
+extern int memcmp_jazz(const uint8_t *, const uint8_t *);
+
+void test_memset_zero_u8(void) {
+    bool debug = true;
+
+    xmss_params p;
+    uint32_t oid;
+
+    if (xmss_str_to_oid(&oid, xstr(IMPL)) == -1) {
+        fprintf(stderr, "Failed to generate oid from impl name\n");
+        exit(-1);
+    }
+
+    if (xmss_parse_oid(&p, oid) == -1) {
+        fprintf(stderr, "Failed to generate params from oid\n");
+        exit(-1);
+    }
+
+    uint8_t buf[p.index_bytes];
+    uint8_t zero_buf[p.index_bytes];
+
+    memset(zero_buf, 0, p.index_bytes * sizeof(uint8_t));
+
+    for (int i = 0; i < TESTS; i++) {
+        if (debug) {
+            printf("[memset_zero_u8] Test %d/%d\n", i + 1, TESTS);
+        }
+
+        randombytes(buf, p.index_bytes * sizeof(uint8_t));
+        memset_zero_u8_jazz(buf);
+        assert(memcmp(buf, zero_buf, p.index_bytes * sizeof(uint8_t)) == 0);
+    }
+}
+
+void test_memset_u8_ptr(void) {
+    bool debug = true;
+
+    uint8_t buf[MAX_BUFSIZE];
+    uint8_t val_buf[MAX_BUFSIZE];
+    uint8_t val;
+
+    for (size_t len = 1; len <= MAX_BUFSIZE; len++) {
+        for (int i = 0; i < TESTS; i++) {
+            if (debug) {
+                printf("[memset_u8 (len=%ld)] Test %d/%d\n", len, i + 1, TESTS);
+            }
+
+            randombytes(&val, sizeof(uint8_t));
+            memset(val_buf, val, len * sizeof(uint8_t));  // setup buffer for comparison
+
+            memset_u8_ptr_jazz(buf, len, val);
+
+            assert(memcmp(buf, val_buf, len * sizeof(uint8_t)) == 0);
+        }
+    }
+}
+
+void test_memcmp(void) {
+    bool debug = true;
+
+    xmss_params p;
+    uint32_t oid;
+
+    if (xmss_str_to_oid(&oid, xstr(IMPL)) == -1) {
+        fprintf(stderr, "Failed to generate oid from impl name\n");
+        exit(-1);
+    }
+
+    if (xmss_parse_oid(&p, oid) == -1) {
+        fprintf(stderr, "Failed to generate params from oid\n");
+        exit(-1);
+    }
+
+    uint8_t a[p.n];
+    uint8_t b[p.n];
+    int res;
+
+    // a and b are random
+    for (int i = 0; i < TESTS; i++) {
+        if (debug) {
+            printf("[memcmp 1] Test %d/%d\n", i + 1, TESTS);
+        }
+
+        randombytes(a, p.n * sizeof(uint8_t));
+        randombytes(b, p.n * sizeof(uint8_t));
+
+        res = memcmp_jazz(a, b);
+
+        assert((memcmp(a, b, p.n * sizeof(uint8_t)) == 0) ? (res == 0) : (res == -1));
+    }
+
+    // a and b are equal
+    for (int i = 0; i < TESTS; i++) {
+        if (debug) {
+            printf("[memcmp 2] Test %d/%d\n", i + 1, TESTS);
+        }
+
+        randombytes(a, p.n * sizeof(uint8_t));
+        memcpy(b, a, p.n * sizeof(uint8_t));  // a and b are equal
+
+        res = memcmp_jazz(a, b);
+
+        assert((memcmp(a, b, p.n * sizeof(uint8_t)) == 0) ? (res == 0) : (res == -1));
+        assert(res == 0);
+    }
+
+    // a and b are not equal
+    for (int i = 0; i < TESTS; i++) {
+        if (debug) {
+            printf("[memcmp 3] Test %d/%d\n", i + 1, TESTS);
+        }
+
+        do {
+            randombytes(a, p.n * sizeof(uint8_t));
+            randombytes(b, p.n * sizeof(uint8_t));
+        } while (memcmp(a, b, p.n * sizeof(uint8_t) == 0));  // make sure a and b are not equal
+
+        res = memcmp_jazz(a, b);
+
+        assert((memcmp(a, b, p.n * sizeof(uint8_t)) == 0) ? (res == 0) : (res == -1));
+        assert(res == -1);
+    }
+}
+
+int main(void) {
+    test_memset_zero_u8();
+    test_memset_u8_ptr();
+    test_memcmp();
+    puts("MEM-* : OK");
+    return 0;
+}
