proof/correctness/Correctness_Hash.ec
@@ -4,11 +4,35 @@ require import AllCore List RealExp IntDiv.
 from Jasmin require import JModel.
 
 require import XMSS_IMPL_PP XMSS_IMPL.
-require import Address Notation Primitives.
+require import Address Notation Primitives XMSS_MT_PRF.
 
-require import Array8 Array32.
+require import Array8 Array32 Array64.
+(*---*) import NBytes.
 
-import NBytes.
+require import Utils. (* valid_ptr *)
+
+pred array32_list_eq (x : W8.t Array32.t) (y : W8.t list) = 
+  forall (k : int), 0 <= k < 32 => x.[k] = nth witness y k.
+
+axiom hash_ptr (mem : global_mem_t) (ptr inlen : W64.t) :
+  array32_list_eq (Hash_ptr ptr inlen) (Hash (mkseq (fun (i : int) => loadW8 mem ((W64.to_uint ptr) + i)) (to_uint inlen))).
+
+
+op addr_to_bytes (a : W32.t Array8.t) : W8.t Array32.t.
+
+(* PRF *)
+(* Spec: op PRF : seed -> adrs -> key. *)
+(* IMPL: op _PRF_ : W8.t Array32.t -> W8.t Array32.t -> W8.t Array32.t -> W8.t Array32.t. *)
+op _PRF_ : W8.t Array32.t -> W8.t Array32.t -> W8.t Array32.t -> W8.t Array32.t.
+
+axiom prf_equiv (out : W8.t Array32.t, addr : W32.t Array8.t, seed : W8.t Array32.t) :
+  PRF (to_list seed) addr = to_list (_PRF_ out (addr_to_bytes addr) seed).
+
+
+(* spec: op F : key -> nbytes -> nbytes. *)
+(* impl: op Hash : W8.t list -> W8.t list.*)
+axiom hash_F_equiv (a : key, b : nbytes) : F a b = Hash (a ++ b).
+
 
 lemma thash_f_correct (_out_ : W8.t Array32.t, _pub_seed_ : W8.t Array32.t, _addr_ : W32.t Array8.t) :
     equiv [Mp(Syscall).__thash_f ~ Chain.thash :
@@ -16,8 +40,28 @@ lemma thash_f_correct (_out_ : W8.t Array32.t, _pub_seed_ : W8.t Array32.t, _add
        res{2}.`1 = to_list res{1}.`1 /\ res{1}.`2 = res{2}.`2].
 proof.
 proc.
-admit.
+auto => />.
+- move => &1 &2 * ; split.
+  + admit.
+  + admit.
+- admit.
 qed.
 
-(* axiom sobre prf keygen *)
-(* axiom sobre prf e F *)
+lemma thash_rand_hash (_out : W8.t Array32.t, _in : W8.t Array64.t, _seed : W8.t Array32.t, _addr : W32.t Array8.t) :
+    hoare[Mp(Syscall).__thash_h : 
+      arg = (_out, _in, _seed, _addr) ==> 
+          res.`1 = Array32.of_list witness (rand_hash (to_list _out) (to_list _in) (to_list _seed) _addr).`1].
+proof.
+proc.
+auto => />.
+- move => &hr H0 addr buf H1. congr. rewrite /rand_hash. admit.
+- while (
+  0 <= to_uint i <= 64
+) ; auto => />.
+    + progress. 
+      * rewrite to_uintD /#.
+      * rewrite to_uintD_small ; smt(@W64).
+    + progress. congr. rewrite /rand_hash. admit.
+    + admit.
+qed.
+
