proof/correctness/Correctness_Address.ec
@@ -7,54 +7,54 @@ from Jasmin require import JModel.
 require import Array8.
 
 require import Address.
-require import XMSS_IMPL.
+require import XMSS_IMPL XMSS_IMPL_PP.
 
-lemma set_layer_addr_op_impl (addr : adrs, layer : int): 
+lemma set_layer_addr_correct (addr : adrs, layer : int): 
     set_layer_addr_pre layer => 
-        hoare[M(Syscall).__set_layer_addr : 
+        hoare[Mp(Syscall).__set_layer_addr : 
             arg = (addr, W32.of_int layer) ==> res = set_layer_addr addr layer].
-proof. move => ?. proc. auto. qed.
+proof. move => ? ; proc ; auto. qed.
 
-lemma set_tree_addr_op_impl (address : adrs, tree_address : int):
+lemma set_tree_addr_correct (address : adrs, tree_address : int):
     set_tree_addr_pre tree_address => 
-        hoare[M(Syscall).__set_tree_addr : 
+        hoare[Mp(Syscall).__set_tree_addr : 
             arg = (address, W64.of_int tree_address) ==> res = set_tree_addr address tree_address].
-proof. move => ?. proc. auto. qed.
+proof. move => ? ; proc ; auto. qed.
 
-lemma set_type_op_impl (address : adrs, _type : int):
+lemma set_type_correct (address : adrs, _type : int):
     set_type_pre _type =>
-        hoare[M(Syscall).__set_type :
+        hoare[Mp(Syscall).__set_type :
             arg = (address, W32.of_int _type) ==> res = set_type address _type].
-proof. move => ?. proc. auto. qed.
+proof. move => ? ; proc ; auto. qed.
 
-lemma set_ots_addr_op_impl (address : adrs, ots_addr : int):
+lemma set_ots_addr_correct (address : adrs, ots_addr : int):
     set_ots_addr_pre ots_addr => 
-        hoare[M(Syscall).__set_ots_addr :
+        hoare[Mp(Syscall).__set_ots_addr :
             arg = (address, W32.of_int ots_addr) ==> res = set_ots_addr address ots_addr].
 proof. move => ?. proc. auto. qed.
 
-lemma set_chain_addr_op_impl (address : adrs, chain_addr : int):
+lemma set_chain_addr_correct (address : adrs, chain_addr : int):
     set_chain_addr_pre chain_addr => 
-        hoare[M(Syscall).__set_chain_addr :
+        hoare[Mp(Syscall).__set_chain_addr :
             arg = (address, W32.of_int chain_addr) ==> res = set_chain_addr address chain_addr].
 proof. move => ?. proc. auto. qed.
 
-lemma set_hash_addr_op_impl (address : adrs, hash_addr : int):
+lemma set_hash_addr_correct (address : adrs, hash_addr : int):
     set_hash_addr_pre hash_addr =>
-        hoare[M(Syscall).__set_hash_addr :
+        hoare[Mp(Syscall).__set_hash_addr :
             arg = (address, W32.of_int hash_addr) ==> res = set_hash_addr address hash_addr].
 proof. move => ?. proc. auto. qed.
 
-lemma set_ltree_addr_op_impl (address : adrs, ltree_addr : int):
+lemma set_ltree_addr_correct (address : adrs, ltree_addr : int):
     set_ltree_addr_pre ltree_addr =>
-        hoare[M(Syscall).__set_ltree_addr :
+        hoare[Mp(Syscall).__set_ltree_addr :
             arg = (address, W32.of_int ltree_addr) ==> 
                 res = set_ltree_addr address ltree_addr].
 proof. move => ?. proc. auto. qed.
 
-lemma set_tree_height_op_impl (address : adrs, tree_height : int):
+lemma set_tree_height_correct (address : adrs, tree_height : int):
     tree_height_pre tree_height =>
-        hoare[M(Syscall).__set_tree_height :
+        hoare[Mp(Syscall).__set_tree_height :
             arg = (address, W32.of_int tree_height) ==> res = set_tree_height address tree_height].
 proof. move => ?. proc. auto. qed.
 
@@ -67,9 +67,9 @@ move => ?.
 smt(@W32).
 qed.
 
-lemma set_tree_index_op_impl (address : adrs, tree_index) : 
+lemma set_tree_index_correct (address : adrs, tree_index) : 
     set_tree_index_pre tree_index => 
-        hoare[M(Syscall).__set_tree_index :
+        hoare[Mp(Syscall).__set_tree_index :
             arg = (address, W32.of_int tree_index) ==> res = set_tree_index address tree_index].
 proof. move => ?. proc. auto. qed.
 
@@ -78,9 +78,9 @@ lemma get_set_tree_index (address : adrs, tree_index : int) :
   get_tree_index (set_tree_index address tree_index) = tree_index.  
 proof. rewrite /get_tree_index /set_tree_index. move => ?. smt(get_setE @W32). qed.
 
-lemma set_key_and_mask_op_impl (address : adrs, key_and_mask : int):
+lemma set_key_and_mask_correct (address : adrs, key_and_mask : int):
     set_key_and_mask_pre key_and_mask =>
-        hoare[M(Syscall).__set_key_and_mask :
+        hoare[Mp(Syscall).__set_key_and_mask :
             arg = (address, W32.of_int key_and_mask) ==> res = set_key_and_mask address key_and_mask].
 proof. move => ?. proc. auto. qed.
 
