proof/extraction/XMSS_IMPL.ec
@@ -961,21 +961,6 @@ module M(SC:Syscall_t) = {
     return (out);
   }
   
-  proc __ull_to_bytes_2 (out:W8.t Array2.t, in_0:W64.t) : W8.t Array2.t = {
-    var aux: int;
-    
-    var i:int;
-    
-    aux <- (- 1);
-    i <- (2 - 1);
-    while (aux < i) {
-      out.[i] <- (truncateu8 in_0);
-      in_0 <- (in_0 `>>` (W8.of_int 8));
-      i <- i - 1;
-    }
-    return (out);
-  }
-  
   proc __ull_to_bytes_4 (out:W8.t Array4.t, in_0:W64.t) : W8.t Array4.t = {
     var aux: int;
     
@@ -998,6 +983,21 @@ module M(SC:Syscall_t) = {
     
     aux <- (- 1);
     i <- (32 - 1);
+    while (aux < i) {
+      out.[i] <- (truncateu8 in_0);
+      in_0 <- (in_0 `>>` (W8.of_int 8));
+      i <- i - 1;
+    }
+    return (out);
+  }
+  
+  proc __ull_to_bytes_2 (out:W8.t Array2.t, in_0:W64.t) : W8.t Array2.t = {
+    var aux: int;
+    
+    var i:int;
+    
+    aux <- (- 1);
+    i <- (2 - 1);
     while (aux < i) {
       out.[i] <- (truncateu8 in_0);
       in_0 <- (in_0 `>>` (W8.of_int 8));
@@ -1128,18 +1128,14 @@ module M(SC:Syscall_t) = {
     return (a);
   }
   
-  proc __memset_u8_ptr (a_ptr:W64.t, inlen:W64.t, value:W8.t) : unit = {
+  proc __memset_u8_ptr (_ptr:W64.t, inlen:W64.t, value:W8.t) : unit = {
     
-    var _ptr:W64.t;
     var i:W64.t;
     
-    _ptr <- a_ptr;
     i <- (W64.of_int 0);
     
     while ((i \ult inlen)) {
-      Glob.mem <-
-      storeW8 Glob.mem (W64.to_uint (_ptr + (W64.of_int 0))) (value);
-      _ptr <- (_ptr + (W64.of_int 1));
+      Glob.mem <- storeW8 Glob.mem (W64.to_uint (_ptr + i)) (value);
       i <- (i + (W64.of_int 1));
     }
     return ();
@@ -1297,8 +1293,8 @@ module M(SC:Syscall_t) = {
     return (out);
   }
   
-  proc __memcpy_u8u8_2_32_2144 (out:W8.t Array32.t, in_0:W8.t Array2144.t,
-                                in_offset:W64.t, bytes:W64.t) : W8.t Array32.t *
+  proc __memcpy_u8u8_2_64_2144 (out:W8.t Array64.t, in_0:W8.t Array2144.t,
+                                in_offset:W64.t, bytes:W64.t) : W8.t Array64.t *
                                                                 W64.t = {
     
     var i:W64.t;
@@ -1313,8 +1309,8 @@ module M(SC:Syscall_t) = {
     return (out, in_offset);
   }
   
-  proc __memcpy_u8u8_2_64_2144 (out:W8.t Array64.t, in_0:W8.t Array2144.t,
-                                in_offset:W64.t, bytes:W64.t) : W8.t Array64.t *
+  proc __memcpy_u8u8_2_32_2144 (out:W8.t Array32.t, in_0:W8.t Array2144.t,
+                                in_offset:W64.t, bytes:W64.t) : W8.t Array32.t *
                                                                 W64.t = {
     
     var i:W64.t;
@@ -1369,22 +1365,6 @@ module M(SC:Syscall_t) = {
     return ();
   }
   
-  proc __memcpy_u8pu8_4 (out:W64.t, offset:W64.t, in_0:W8.t Array4.t) : 
-  W64.t * W64.t = {
-    
-    var i:W64.t;
-    
-    i <- (W64.of_int 0);
-    
-    while ((i \ult (W64.of_int 4))) {
-      Glob.mem <-
-      storeW8 Glob.mem (W64.to_uint (out + offset)) (in_0.[(W64.to_uint i)]);
-      offset <- (offset + (W64.of_int 1));
-      i <- (i + (W64.of_int 1));
-    }
-    return (out, offset);
-  }
-  
   proc __memcpy_u8pu8_32 (out:W64.t, offset:W64.t, in_0:W8.t Array32.t) : 
   W64.t * W64.t = {
     
@@ -1401,12 +1381,19 @@ module M(SC:Syscall_t) = {
     return (out, offset);
   }
   
-  proc _memcpy_u8pu8_4 (out:W64.t, offset:W64.t, in_0:W8.t Array4.t) : 
+  proc __memcpy_u8pu8_4 (out:W64.t, offset:W64.t, in_0:W8.t Array4.t) : 
   W64.t * W64.t = {
     
+    var i:W64.t;
     
+    i <- (W64.of_int 0);
     
-    (out, offset) <@ __memcpy_u8pu8_4 (out, offset, in_0);
+    while ((i \ult (W64.of_int 4))) {
+      Glob.mem <-
+      storeW8 Glob.mem (W64.to_uint (out + offset)) (in_0.[(W64.to_uint i)]);
+      offset <- (offset + (W64.of_int 1));
+      i <- (i + (W64.of_int 1));
+    }
     return (out, offset);
   }
   
@@ -1419,17 +1406,12 @@ module M(SC:Syscall_t) = {
     return (out, offset);
   }
   
-  proc _x_memcpy_u8pu8_4 (out:W64.t, offset:W64.t, in_0:W8.t Array4.t) : 
+  proc _memcpy_u8pu8_4 (out:W64.t, offset:W64.t, in_0:W8.t Array4.t) : 
   W64.t * W64.t = {
     
     
     
-    out <- out;
-    offset <- offset;
-    in_0 <- in_0;
-    (out, offset) <@ _memcpy_u8pu8_4 (out, offset, in_0);
-    out <- out;
-    offset <- offset;
+    (out, offset) <@ __memcpy_u8pu8_4 (out, offset, in_0);
     return (out, offset);
   }
   
@@ -1447,16 +1429,28 @@ module M(SC:Syscall_t) = {
     return (out, offset);
   }
   
+  proc _x_memcpy_u8pu8_4 (out:W64.t, offset:W64.t, in_0:W8.t Array4.t) : 
+  W64.t * W64.t = {
+    
+    
+    
+    out <- out;
+    offset <- offset;
+    in_0 <- in_0;
+    (out, offset) <@ _memcpy_u8pu8_4 (out, offset, in_0);
+    out <- out;
+    offset <- offset;
+    return (out, offset);
+  }
+  
   proc _zero_address (addr:W32.t Array8.t) : W32.t Array8.t = {
     var aux: int;
     
     var i:int;
     
     i <- 0;
-    while (i < 4) {
-      addr <-
-      Array8.init
-      (WArray32.get32 (WArray32.set64 (WArray32.init32 (fun i_0 => (addr).[i_0])) i ((W64.of_int 0))));
+    while (i < 8) {
+      addr.[i] <- (W32.of_int 0);
       i <- i + 1;
     }
     return (addr);
@@ -2065,40 +2059,6 @@ module M(SC:Syscall_t) = {
     return (out, addr);
   }
   
-  proc __base_w_3_2 (output:W32.t Array3.t, input:W8.t Array2.t) : W32.t Array3.t = {
-    
-    var in_0:W64.t;
-    var bits:W64.t;
-    var total:W32.t;
-    var i:W64.t;
-    var _of_:bool;
-    var _cf_:bool;
-    var _sf_:bool;
-    var _zf_:bool;
-    var  _0:bool;
-    
-    in_0 <- (W64.of_int 0);
-    bits <- (W64.of_int 0);
-    total <- (W32.of_int 0);
-    i <- (W64.of_int 0);
-    
-    while ((i \ult (W64.of_int 3))) {
-      if ((bits = (W64.of_int 0))) {
-        total <- (zeroextu32 input.[(W64.to_uint in_0)]);
-        in_0 <- (in_0 + (W64.of_int 1));
-        bits <- (bits + (W64.of_int 8));
-      } else {
-        
-      }
-      bits <- (bits - (W64.of_int 4));
-      (_of_, _cf_, _sf_,  _0, _zf_, total) <- SHR_32 total (truncateu8 bits);
-      total <- (total `&` (W32.of_int (16 - 1)));
-      output.[(W64.to_uint i)] <- total;
-      i <- (i + (W64.of_int 1));
-    }
-    return (output);
-  }
-  
   proc __base_w_67_32 (output:W32.t Array67.t, input:W8.t Array32.t) : 
   W32.t Array67.t = {
     
@@ -2118,6 +2078,40 @@ module M(SC:Syscall_t) = {
     i <- (W64.of_int 0);
     
     while ((i \ult (W64.of_int 67))) {
+      if ((bits = (W64.of_int 0))) {
+        total <- (zeroextu32 input.[(W64.to_uint in_0)]);
+        in_0 <- (in_0 + (W64.of_int 1));
+        bits <- (bits + (W64.of_int 8));
+      } else {
+        
+      }
+      bits <- (bits - (W64.of_int 4));
+      (_of_, _cf_, _sf_,  _0, _zf_, total) <- SHR_32 total (truncateu8 bits);
+      total <- (total `&` (W32.of_int (16 - 1)));
+      output.[(W64.to_uint i)] <- total;
+      i <- (i + (W64.of_int 1));
+    }
+    return (output);
+  }
+  
+  proc __base_w_3_2 (output:W32.t Array3.t, input:W8.t Array2.t) : W32.t Array3.t = {
+    
+    var in_0:W64.t;
+    var bits:W64.t;
+    var total:W32.t;
+    var i:W64.t;
+    var _of_:bool;
+    var _cf_:bool;
+    var _sf_:bool;
+    var _zf_:bool;
+    var  _0:bool;
+    
+    in_0 <- (W64.of_int 0);
+    bits <- (W64.of_int 0);
+    total <- (W32.of_int 0);
+    i <- (W64.of_int 0);
+    
+    while ((i \ult (W64.of_int 3))) {
       if ((bits = (W64.of_int 0))) {
         total <- (zeroextu32 input.[(W64.to_uint in_0)]);
         in_0 <- (in_0 + (W64.of_int 1));
