scripts/run-all-tests.sh
@@ -1,12 +1,17 @@
 #!/bin/bash
 
 test_dirs=(
-    "wots"
-    "xmss"
+    "hash_address"
+    "stdlib"
+    "sha256/sha256_array"
+    "sha256/sha256_in_ptr"
+    "hash"
+    # "wots"
+    # "xmss"
 )
 
 for dir in ${test_dirs[@]}; do
-    make -C ../test/$dir clean
-    make -C ../test/$dir
-    make -C ../test/$dir run
+    make     -C ../test/$dir clean
+    make -j8 -C ../test/$dir
+    make -j8 -C ../test/$dir run
 done
